core/Data.thy
@@ -7,24 +7,116 @@ datatype 'l uid = U (label:\<open>'l\<close>) (id:\<open>nat\<close>)
 
 instantiation uid :: (linorder) linorder
 begin
-fun less_uid where
-   \<open>less_uid (U i1 id1) (U i2 id2) = (i1 < i2 \<or> (i1 = i2 \<and> id1 < id2))\<close>
-instance sorry
+definition less_uid where
+   \<open>less_uid \<equiv> \<lambda>(U i1 id1) \<Rightarrow> \<lambda>(U i2 id2) \<Rightarrow> (i1 < i2 \<or> (i1 = i2 \<and> id1 < id2))\<close>
+
+definition less_eq_uid where
+   \<open>less_eq_uid \<equiv> \<lambda>(U i1 id1) \<Rightarrow> \<lambda>(U i2 id2) \<Rightarrow> (i1 < i2 \<or> (i1 = i2 \<and> id1 \<le> id2))\<close>
+
+instance
+  by standard (auto simp: less_uid_def less_eq_uid_def split: uid.splits)
+
 end
+
+lemma less_uid_simp[simp]:
+  \<open>(U i1 id1) < (U i2 id2) = (i1 < i2 \<or> (i1 = i2 \<and> id1 < id2))\<close>
+  unfolding less_uid_def by simp
+
+lemma less_eq_uid_simp[simp]:
+  \<open>(U i1 id1) \<le> (U i2 id2) = (i1 < i2 \<or> (i1 = i2 \<and> id1 \<le> id2))\<close>
+  unfolding less_eq_uid_def by simp
 
 datatype 'l ptr = Leaf \<open>bool\<close> | Node \<open>'l uid\<close>
 
+instantiation ptr :: (linorder) linorder
+begin
+fun less_ptr where
+  \<open>less_ptr (Node u1) (Node u2) \<longleftrightarrow> u1 < u2\<close>
+| \<open>less_ptr (Node _) (Leaf _) \<longleftrightarrow> True\<close>
+| \<open>less_ptr (Leaf _) (Node _) \<longleftrightarrow> False\<close>
+| \<open>less_ptr (Leaf b1) (Leaf b2) \<longleftrightarrow> b1 < b2\<close>
+
+lemma less_ptr_alt_def:
+  "(ptr1 :: ('b :: linorder) ptr) < (ptr2 :: ('b :: linorder) ptr) = (case (ptr1, ptr2) of
+    (Node u1, Node u2) \<Rightarrow> u1 < u2
+  | (Node _, Leaf _) \<Rightarrow> True
+  | (Leaf _, Node _) \<Rightarrow> False
+  | (Leaf b1, Leaf b2) \<Rightarrow> b1 < b2
+)"
+  by (cases "(ptr1, ptr2)" rule: less_ptr.cases) auto
+
+definition less_eq_ptr where
+  "less_eq_ptr (ptr1 :: ('b :: linorder) ptr) (ptr2 :: ('b :: linorder) ptr) = (case (ptr1, ptr2) of
+    (Node u1, Node u2) \<Rightarrow> u1 \<le> u2
+  | (Node _, Leaf _) \<Rightarrow> True
+  | (Leaf _, Node _) \<Rightarrow> False
+  | (Leaf b1, Leaf b2) \<Rightarrow> b1 \<le> b2
+)"
+
+instance
+  by standard
+     (auto split: ptr.splits simp del: less_ptr.simps simp add: less_ptr_alt_def less_eq_ptr_def)
+end
+
 datatype 'l node = N (uid:\<open>'l uid\<close>) (low:\<open>'l ptr\<close>) (high:\<open>'l ptr\<close>)
+
+instantiation node :: (linorder) linorder
+begin
+definition less_node where
+  \<open>less_node \<equiv> \<lambda>(N i1 t1 e1) \<Rightarrow> \<lambda>(N i2 t2 e2) \<Rightarrow>
+    (i1 < i2 \<or> i1 = i2 \<and> e1 < e2 \<or> i1 = i2 \<and> e1 = e2 \<and> t1 < t2)\<close>
+
+definition less_eq_node where
+  \<open>less_eq_node \<equiv> \<lambda>(N i1 t1 e1) \<Rightarrow> \<lambda>(N i2 t2 e2) \<Rightarrow>
+    (i1 < i2 \<or> i1 = i2 \<and> e1 < e2 \<or> i1 = i2 \<and> e1 = e2 \<and> t1 \<le> t2)\<close>
+
+instance
+  by standard (auto simp: less_node_def less_eq_node_def split: node.splits)
+
+end
+
+lemma less_node_simp[simp]:
+  \<open>(N i1 t1 e1) < (N i2 t2 e2) =
+    (i1 < i2 \<or> i1 = i2 \<and> e1 < e2 \<or> i1 = i2 \<and> e1 = e2 \<and> t1 < t2)\<close>
+  unfolding less_node_def by simp
+
+lemma less_eq_node_simp[simp]:
+  \<open>(N i1 t1 e1) \<le> (N i2 t2 e2) \<longleftrightarrow>
+    (i1 < i2 \<or> i1 = i2 \<and> e1 < e2 \<or> i1 = i2 \<and> e1 = e2 \<and> t1 \<le> t2)\<close>
+  unfolding less_eq_node_def by simp
+
 
 datatype 'l bdd = Constant \<open>bool\<close> | Nodes \<open>'l node list\<close>
 
 type_synonym 'l assignment = \<open>'l \<Rightarrow> bool\<close>
 
-fun well_formed_nl :: \<open>'l node list \<Rightarrow> bool\<close> where
-  \<open>well_formed_nl []             = True\<close>
-| \<open>well_formed_nl (N i t e # ns) = (well_formed_nl ns
-                                    \<and> (case t of Leaf b \<Rightarrow> True | Node l_uid \<Rightarrow> \<exists>n \<in> set ns . uid n = l_uid)
-                                    \<and> (case e of Leaf b \<Rightarrow> True | Node h_uid \<Rightarrow> \<exists>n \<in> set ns . uid n = h_uid))\<close>
+fun closed :: \<open>'l node list \<Rightarrow> bool\<close> where
+  \<open>closed []             = True\<close>
+| \<open>closed (N i t e # ns) = (closed ns
+                          \<and> (case t of Leaf b \<Rightarrow> True | Node l_uid \<Rightarrow> \<exists>n \<in> set ns . uid n = l_uid)
+                          \<and> (case e of Leaf b \<Rightarrow> True | Node h_uid \<Rightarrow> \<exists>n \<in> set ns . uid n = h_uid))\<close>
+
+definition
+  "ptr_lb i \<equiv> \<lambda>Node n \<Rightarrow> i < label n | _ \<Rightarrow> True"
+
+fun inc_labels :: \<open>('l::linorder) node list \<Rightarrow> bool\<close> where
+  \<open>inc_labels []             \<longleftrightarrow> True\<close>
+| \<open>inc_labels (N i t e # ns) \<longleftrightarrow> inc_labels ns \<and> ptr_lb (label i) t \<and> ptr_lb (label i) e\<close>
+
+definition
+  "well_formed_nl ns \<equiv> closed ns \<and> inc_labels ns \<and> sorted ns"
+
+lemma closed_if_well_formed_nl[intro,simp]:
+  "closed ns" if "well_formed_nl ns"
+  using that unfolding well_formed_nl_def ..
+
+lemma inc_labels_if_well_formed_nl[intro,simp]:
+  "inc_labels ns" if "well_formed_nl ns"
+  using that unfolding well_formed_nl_def by (elim conjE)
+
+lemma sorted_if_well_formed_nl[intro,simp]:
+  "sorted ns" if "well_formed_nl ns"
+  using that unfolding well_formed_nl_def by (elim conjE)
 
 lemma nl_induct[case_names Nil Cons]:
   fixes P :: "'a node list \<Rightarrow> bool"
@@ -32,9 +124,9 @@ lemma nl_induct[case_names Nil Cons]:
   assumes "P []"
     and "\<And>i t e ns. P ns \<Longrightarrow> P (N i t e # ns)"
   shows "P ns"
-  using assms by (rule Data.well_formed_nl.induct)
+  using assms by (rule closed.induct)
 
-fun well_formed :: \<open>'l bdd \<Rightarrow> bool\<close> where
+fun well_formed :: \<open>('l::linorder) bdd \<Rightarrow> bool\<close> where
   \<open>well_formed (Constant _) = True\<close>
 | \<open>well_formed (Nodes [])   = False\<close>
 | \<open>well_formed (Nodes ns)   = well_formed_nl ns\<close>
