core/Evaluate.thy
@@ -4,13 +4,16 @@ imports ROBDD.BDT Data
 begin
 text \<open> Stream-like evaluation of Adiar's BDD representation \<close>
 
-fun bdd_eval_node :: \<open>'l node list \<Rightarrow> 'l assignment \<Rightarrow> 'l uid \<Rightarrow> bool\<close> where
+fun bdd_eval_node :: \<open>'l node list \<Rightarrow> 'l assignment \<Rightarrow> 'l uid \<Rightarrow> bool\<close>
+and bdd_eval_ptr :: \<open>'l node list \<Rightarrow> 'l assignment \<Rightarrow> 'l ptr \<Rightarrow> bool\<close>
+  where
   \<open>bdd_eval_node []     _ _ = undefined\<close>
 | \<open>bdd_eval_node (n#ns) a t = (if uid n = t
                               then let child = (if a (label t) then high n else low n)
-                                   in (case child of Leaf b \<Rightarrow> b
-                                                   | Node t' \<Rightarrow> bdd_eval_node ns a t' )
+                                   in bdd_eval_ptr ns a child
                               else bdd_eval_node ns a t)\<close>
+| \<open>bdd_eval_ptr ns a (Leaf b) = b\<close>
+| \<open>bdd_eval_ptr ns a (Node t) = bdd_eval_node ns a t\<close>
 
 fun bdd_eval :: \<open>'l bdd \<Rightarrow> 'l assignment \<Rightarrow> bool\<close> where
   \<open>bdd_eval (Constant b)        _ = b\<close>
@@ -22,25 +25,25 @@ text \<open> Linking to Binary Decision Tree \<close>
 abbreviation Ifleaf_of_leaf :: \<open>bool \<Rightarrow> 'l ifex\<close> where
   \<open>Ifleaf_of_leaf b \<equiv> (if b then Trueif else Falseif)\<close>
 
-fun bdt_of_bdd_node :: \<open>'l node list \<Rightarrow> 'l uid \<Rightarrow> 'l ifex\<close> where
-  \<open>bdt_of_bdd_node []     _ = undefined\<close>
-| \<open>bdt_of_bdd_node (n#ns) t = (if uid n = t
+fun bdt_of_node :: \<open>'l node list \<Rightarrow> 'l uid \<Rightarrow> 'l ifex\<close> where
+  \<open>bdt_of_node []     _ = undefined\<close>
+| \<open>bdt_of_node (n#ns) t = (if uid n = t
                                then let high_subtree = (case high n of Leaf b \<Rightarrow> Ifleaf_of_leaf b
-                                                                    | Node t' \<Rightarrow> bdt_of_bdd_node ns t')
+                                                                    | Node t' \<Rightarrow> bdt_of_node ns t')
                                       ; low_subtree = (case low n of Leaf b \<Rightarrow> Ifleaf_of_leaf b
-                                                                  | Node t' \<Rightarrow> bdt_of_bdd_node ns t')
+                                                                  | Node t' \<Rightarrow> bdt_of_node ns t')
                                      in IF (label t) high_subtree low_subtree
-                               else bdt_of_bdd_node ns t)\<close>
+                               else bdt_of_node ns t)\<close>
 
 fun bdt_of_bdd :: \<open>'l bdd \<Rightarrow> 'l ifex\<close> where
   \<open>bdt_of_bdd (Constant b) = Ifleaf_of_leaf b\<close>
-| \<open>bdt_of_bdd (Nodes (root#ns)) = bdt_of_bdd_node (root#ns) (uid root)\<close>
+| \<open>bdt_of_bdd (Nodes (root#ns)) = bdt_of_node (root#ns) (uid root)\<close>
 | \<open>bdt_of_bdd (Nodes []) = undefined\<close>
 
 
 lemma bdd_eval_node_iff_val_ifex_aux:
-  assumes \<open>well_formed_nl ns\<close> \<open>t \<in> uid ` set ns\<close>
-  shows \<open>bdd_eval_node ns a t \<longleftrightarrow> val_ifex (bdt_of_bdd_node ns t) a\<close>
+  assumes \<open>closed ns\<close> \<open>t \<in> uid ` set ns\<close>
+  shows \<open>bdd_eval_node ns a t \<longleftrightarrow> val_ifex (bdt_of_node ns t) a\<close>
   using assms
 proof (induction ns arbitrary: t rule: nl_induct)
   case (Cons i t e ns)
@@ -54,20 +57,58 @@ theorem bdd_eval_iff_val_ifex:
 proof (cases bdd rule: bdd_cases)
   case (Nodes i t e ns)
   with assms show ?thesis
-    by (auto split:ptr.splits
-             dest:imageI[where f = uid] bdd_eval_node_iff_val_ifex_aux[where a = a])
+    by (auto split: ptr.splits
+             dest:  imageI[where f = uid] bdd_eval_node_iff_val_ifex_aux[where a = a]
+             dest!: closed_if_well_formed_nl)
 qed (use assms in auto)
 
 text \<open>Evaluation of pointers, this comes in handy later.\<close>
-fun bdd_eval_ptr :: \<open>'l node list \<Rightarrow> 'l assignment \<Rightarrow> 'l ptr \<Rightarrow> bool\<close> where
-  \<open>bdd_eval_ptr ns a (Leaf b) = b\<close>
-| \<open>bdd_eval_ptr ns a (Node t) = bdd_eval_node ns a t\<close>
 
-lemma bdd_eval_node_Cons_alt:
-  \<open>bdd_eval_node (n#ns) a t = (if uid n = t
-                              then let child = (if a (label t) then high n else low n)
-                                   in bdd_eval_ptr ns a child
-                              else bdd_eval_node ns a t)\<close>
-  unfolding bdd_eval_node.simps by (simp split: ptr.splits)
+fun bdt_of_ptr :: \<open>'l node list \<Rightarrow> 'l ptr \<Rightarrow> 'l ifex\<close> where
+  \<open>bdt_of_ptr ns (Leaf b) = Ifleaf_of_leaf b\<close>
+| \<open>bdt_of_ptr ns (Node u) = bdt_of_node ns u\<close>
+
+lemma bdt_of_node_Cons_alt:
+  \<open>bdt_of_node (n#ns) t = (if uid n = t
+                               then let high_subtree = bdt_of_ptr ns (high n)
+                                      ; low_subtree = bdt_of_ptr ns (low n)
+                                     in IF (label t) high_subtree low_subtree
+                               else bdt_of_node ns t)\<close>
+  by (simp split: ptr.split)
+
+fun vars_of_bdt where
+  "vars_of_bdt (IF i t e) = insert i (vars_of_bdt t \<union> vars_of_bdt e)"
+| "vars_of_bdt _ = {}"
+
+definition dom_bounded_vars where
+  "dom_bounded_vars S a \<equiv> \<forall>x. x \<notin> S \<longrightarrow> a x = False"
+
+definition
+  "vars_of_bdd bdd = vars_of_bdt (bdt_of_bdd bdd)"
+
+definition
+  "vars_of_node ns node = vars_of_bdt (bdt_of_node ns node)"
+
+definition
+  "vars_of_ptr ns ptr = vars_of_bdt (bdt_of_ptr ns ptr)"
+
+definition
+  "num_assignments_vars bdd = card {a. bdd_eval bdd a \<and> dom_bounded_vars (vars_of_bdd bdd) a}"
+
+definition
+  "num_assignments_vars_ptr ns ptr =
+    card {a. bdd_eval_ptr ns a ptr \<and> dom_bounded_vars (vars_of_ptr ns ptr) a}"
+
+definition
+  "num_assignments_vars_node ns node =
+    card {a. bdd_eval_node ns a node \<and> dom_bounded_vars (vars_of_node ns node) a}"
+
+lemma vars_of_bdd_to_node[simp]:
+  "vars_of_bdd (Nodes (N i t e # ns)) = vars_of_node (N i t e # ns) i"
+  unfolding vars_of_bdd_def vars_of_node_def by simp
+
+lemma num_assignments_vars_to_node[simp]:
+  "num_assignments_vars (Nodes (N i t e # ns)) = num_assignments_vars_node (N i t e # ns) i"
+  unfolding num_assignments_vars_def num_assignments_vars_node_def by simp
 
 end
